DemoCoBRA.v
@@ -1,0 +1,60 @@
+Require Import String List.
+Require Import Ast EvalE.
+
+Import ListNotations.
+
+Import BaseTypes.
+Import StdLib.
+
+Definition negb_app_true :=
+    [| (\x : Bool ->
+           case x : Bool return Bool of
+           | true -> false
+           | false -> true) true
+     |].
+
+Print negb_app_true.
+
+Unset Printing Notations.
+Print negb_app_true.
+
+Set Printing Notations.
+
+Import InterpreterEnvList.
+
+(* Execute the program using the interpreter *)
+Compute (expr_eval_n 3 Σ [] negb_app_true).
+
+(* Execute the "indexified", i.e. nameless, program *)
+Compute (expr_eval_i 3 Σ [] (indexify [] negb_app_true)).
+
+Notation plus := "plus".
+
+Definition plus_syn : expr :=
+  [| fix plus (x : Nat) : Nat -> Nat :=
+           case x : Nat return Nat -> Nat of
+           | Z -> \y : Nat -> y
+           | Suc y -> \z : Nat -> Suc (plus y z) |].
+
+Definition two :=
+  (vConstr Nat "Suc"
+           [vConstr Nat "Suc" [vConstr Nat "Z" []]]).
+
+Definition one_plus_one :=
+  [| {plus_syn} 1 1 |].
+
+Compute (expr_eval_n 10 Σ [] [| {plus_syn} 1 1 |]).
+
+Example one_plus_one_two : expr_eval_n 10 Σ [] one_plus_one = Ok two.
+Proof. reflexivity. Qed.
+
+(* Unquote the translated expression *)
+Make Definition my_plus :=
+  Eval compute in (expr_to_term Σ (indexify [] plus_syn)).
+
+Print my_plus.
+
+(* our plus program corresponds to the addition of natural numbers *)
+Lemma my_plus_correct n m :
+  my_plus n m = n + m.
+Proof. induction n;simpl;auto. Qed.
