MyEnv.v
@@ -1,0 +1,45 @@
+Require Import List String.
+
+Import ListNotations.
+
+Definition env (A : Type) := list (string * A).
+
+(** Lookup by variable name *)
+Fixpoint lookup {A} (ρ : env A) (key : string) : option A :=
+  match ρ with
+  | [] => None
+  | (nm,a) :: ρ' =>
+    if (eqb nm key) then Some a else lookup ρ' key
+  end.
+
+Fixpoint lookup_with_ind_rec {A} (i : nat) (ρ : env A) (key : string) : option (nat * A) :=
+  match ρ with
+  | [] => None
+  | (nm,a) :: ρ' =>
+    if (eqb nm key) then Some (i,a)
+    else lookup_with_ind_rec (1+i) ρ' key
+  end.
+
+Definition lookup_with_ind {A} (ρ : env A) (key : string)
+  : option (nat * A) := lookup_with_ind_rec 0 ρ key.
+
+
+  (** Lookup by index (similar to [List.nth_error], but defined by recursion on env *)
+Fixpoint lookup_i {A} (ρ : env A) (i : nat) : option A :=
+  match ρ with
+  | [] => None
+  | (nm,a) :: ρ' =>
+    if (Nat.eqb i 0) then Some a else lookup_i ρ' (i-1)
+  end.
+
+  (** A value environment lookup: *)
+Notation "ρ # '(' k ')'" := (lookup ρ k) (at level 10).
+(** A value environment extension: *)
+Notation "ρ # [ k ~> v ]" := ( (k,v) :: ρ) (at level 50).
+
+Fixpoint remove_by_key {A} (key : string) (ρ : env A) : env A :=
+  match ρ with
+  | [] => []
+  | (nm,a) :: ρ' => if (eqb nm key) then remove_by_key key ρ'
+                  else (nm,a) :: (remove_by_key key ρ')
+  end.
